full verification of clausification

LeanHammer/Rules/Clausification.lean
@@ -91,6 +91,48 @@ theorem clausify_exists_false {p : α → Prop} (x : α) (h : (∃ x, p x) = Fal
 theorem ex_eq_true_of_ex_eq_true {p : α → Prop} (h : (∃ x, p x) = True) : ∃ x, (p x = True) :=
   (of_eq_true h).elim fun a ha => ⟨a, eq_true ha⟩
 
+-- theorem xxx {p : α → Prop} (h : (∃ x, p x) = True ∨ q) : ∃ x, (p x = True) :=
+--   (of_eq_true h).elim fun a ha => ⟨a, eq_true ha⟩
+
+--TODO: generalize `orIntro` + `orCases` & use everywhere
+/-- Construct a proof of 
+ `∃ a, lits[0] ∨ ... ∨ lits[i-1] ∨ lits[i+1] ∨ ... ∨ lits[n] ∨ p a = True` 
+ from a proof of
+`lits[0] ∨ ... ∨ (∃ a, p a) = True ∨ ... ∨ lits[n]`-/
+def existsClause (lits : Array Expr) (i : Nat) (p : Expr) (ty : Expr) (pr : Expr) : MetaM Expr := do
+  Meta.withLocalDeclD `a ty fun a => do
+    let mut resLits := #[]
+    for j in [:lits.size] do
+      if j != i then
+        resLits := resLits.push lits[j]
+    resLits := resLits.push $ p.instantiate1 a
+
+    let mut caseProofs := #[]
+    for j in [:lits.size] do
+      let lit := lits[j]
+      let pr ← Meta.withLocalDeclD `h lit fun h => do
+        if j == i then
+          Meta.mkLambdaFVars #[h] $ ← orIntro resLits (lits.size - 1) (mkApp pr h)
+        else
+          let idx := if j ≥ i then j - 1 else j
+          Meta.mkLambdaFVars #[h] $ ← orIntro resLits idx h
+      caseProofs := caseProofs.push $ pr
+
+    let r ← orCases lits caseProofs
+
+    return ← Meta.mkAppM ``Exists.intro #[a, pr]
+
+
+--TODO: move
+noncomputable def Inhabited.some [Inhabited α] (p : α → Prop) :=
+  let _ : Decidable (∃ a, p a) := Classical.propDecidable _
+  if hp: ∃ a, p a then Classical.choose hp else Inhabited.default
+
+theorem Inhabited.some_spec [Inhabited α] {p : α → Prop} (hp : ∃ a, p a) : 
+  p (Inhabited.some p) := by
+  simp only [Inhabited.some, hp]
+  exact Classical.choose_spec _
+
 def clausificationStepE (e : Expr) (sign : Bool) (c : MClause) (i : Nat) : 
     RuleM (SimpResult (List (MClause × Option (Expr → MetaM Expr)))) := do
   match sign, e with
@@ -137,7 +179,8 @@ def clausificationStepE (e : Expr) (sign : Bool) (c : MClause) (i : Nat) :
     let pr : Expr → MetaM Expr := fun premise => do
       let mvar ← Meta.mkFreshExprMVar ty
       -- TODO: Decompose Or
-      return ← Meta.mkAppM ``Classical.choose_spec #[← Meta.mkAppM ``ex_eq_true_of_ex_eq_true #[premise]]
+      return ← Meta.mkAppM ``eq_true
+        #[← Meta.mkAppM ``Inhabited.some_spec #[← Meta.mkAppM ``of_eq_true #[premise]]]
     Applied [(MClause.mk #[Lit.fromExpr $ b.instantiate1 skTerm], some pr)]
   | false, Expr.app (Expr.app (Expr.const ``And _ _) e₁ _) e₂ _  => 
     let pr : Expr → MetaM Expr := fun premise => do
@@ -198,7 +241,9 @@ where
       trace[Meta.debug] "##B {b}"
       trace[Meta.debug] "##PRTS {parents}"
       -- TODO: Unfold Or
-      return ← Meta.mkAppM ``Classical.choose #[← Meta.mkAppM ``ex_eq_true_of_ex_eq_true #[parents[0]]]
+      let d ← Meta.mkAppM ``Inhabited.some #[mkLambda `x BinderInfo.default ty b]
+      trace[Meta.debug] "##D {d}"
+      return d
     let fvar ← mkFreshSkolem `sk skTy mkProof
     mkAppN fvar (mVarIds.map mkMVar)
   clausifyExists ty b := do
@@ -222,7 +267,7 @@ def clausificationStepLit (c : MClause) (i : Nat) : RuleM (SimpResult (List (MCl
   | _ => return Unapplicable
 -- TODO: True/False on left-hand side?
 
--- TODO: Proof reconstruction
+
 def clausificationStep : MSimpRule := fun c => do
   for i in [:c.lits.size] do
     match ← clausificationStepLit c i with
@@ -257,7 +302,7 @@ def clausificationStep : MSimpRule := fun c => do
                     Meta.mkLambdaFVars #[h] $ ← orIntro (resLits.map Lit.toExpr) idx h
                 caseProofs := caseProofs.push $ pr
 
-              let r ← orCases (← parentLits.map Lit.toExpr) body caseProofs
+              let r ← orCases (← parentLits.map Lit.toExpr) caseProofs
               trace[Meta.debug] "###RES {res}"
               trace[Meta.debug] "###R {← Meta.inferType r}"
               let r ← Meta.mkLambdaFVars xs $ mkApp r appliedPremise
